LeanProofs/.lake/build/ir/LeanProofs/exprDeterminism.c
@@ -1,0 +1,159 @@
+// Lean compiler output
+// Module: LeanProofs.exprDeterminism
+// Imports: public import Init public meta import Init public import LeanProofs.Basic
+#include <lean/lean.h>
+#if defined(__clang__)
+#pragma clang diagnostic ignored "-Wunused-parameter"
+#pragma clang diagnostic ignored "-Wunused-label"
+#elif defined(__GNUC__) && !defined(__CLANG__)
+#pragma GCC diagnostic ignored "-Wunused-parameter"
+#pragma GCC diagnostic ignored "-Wunused-label"
+#pragma GCC diagnostic ignored "-Wunused-but-set-variable"
+#endif
+#ifdef __cplusplus
+extern "C" {
+#endif
+LEAN_EXPORT lean_object* lp_LeanProofs___private_LeanProofs_exprDeterminism_0__evalExpr_match__1_splitter___redArg(lean_object*, lean_object*, lean_object*, lean_object*, lean_object*);
+LEAN_EXPORT lean_object* lp_LeanProofs___private_LeanProofs_exprDeterminism_0__evalExpr_match__1_splitter(lean_object*, lean_object*, lean_object*, lean_object*, lean_object*, lean_object*);
+LEAN_EXPORT lean_object* lp_LeanProofs___private_LeanProofs_exprDeterminism_0__evalExpr_match__1_splitter___redArg(lean_object* v_e_1_, lean_object* v_h__1_2_, lean_object* v_h__2_3_, lean_object* v_h__3_4_, lean_object* v_h__4_5_){
+_start:
+{
+switch(lean_obj_tag(v_e_1_))
+{
+case 0:
+{
+lean_object* v_a_6_; lean_object* v___x_7_; 
+lean_dec(v_h__4_5_);
+lean_dec(v_h__3_4_);
+lean_dec(v_h__2_3_);
+v_a_6_ = lean_ctor_get(v_e_1_, 0);
+lean_inc(v_a_6_);
+lean_dec_ref_known(v_e_1_, 1);
+v___x_7_ = lean_apply_1(v_h__1_2_, v_a_6_);
+return v___x_7_;
+}
+case 1:
+{
+lean_object* v_a_8_; lean_object* v___x_9_; 
+lean_dec(v_h__4_5_);
+lean_dec(v_h__3_4_);
+lean_dec(v_h__1_2_);
+v_a_8_ = lean_ctor_get(v_e_1_, 0);
+lean_inc_ref(v_a_8_);
+lean_dec_ref_known(v_e_1_, 1);
+v___x_9_ = lean_apply_1(v_h__2_3_, v_a_8_);
+return v___x_9_;
+}
+case 2:
+{
+lean_object* v_a_10_; lean_object* v_a_11_; lean_object* v___x_12_; 
+lean_dec(v_h__4_5_);
+lean_dec(v_h__2_3_);
+lean_dec(v_h__1_2_);
+v_a_10_ = lean_ctor_get(v_e_1_, 0);
+lean_inc_ref(v_a_10_);
+v_a_11_ = lean_ctor_get(v_e_1_, 1);
+lean_inc_ref(v_a_11_);
+lean_dec_ref_known(v_e_1_, 2);
+v___x_12_ = lean_apply_2(v_h__3_4_, v_a_10_, v_a_11_);
+return v___x_12_;
+}
+default: 
+{
+lean_object* v_a_13_; lean_object* v_a_14_; lean_object* v___x_15_; 
+lean_dec(v_h__3_4_);
+lean_dec(v_h__2_3_);
+lean_dec(v_h__1_2_);
+v_a_13_ = lean_ctor_get(v_e_1_, 0);
+lean_inc_ref(v_a_13_);
+v_a_14_ = lean_ctor_get(v_e_1_, 1);
+lean_inc_ref(v_a_14_);
+lean_dec_ref_known(v_e_1_, 2);
+v___x_15_ = lean_apply_2(v_h__4_5_, v_a_13_, v_a_14_);
+return v___x_15_;
+}
+}
+}
+}
+LEAN_EXPORT lean_object* lp_LeanProofs___private_LeanProofs_exprDeterminism_0__evalExpr_match__1_splitter(lean_object* v_motive_16_, lean_object* v_e_17_, lean_object* v_h__1_18_, lean_object* v_h__2_19_, lean_object* v_h__3_20_, lean_object* v_h__4_21_){
+_start:
+{
+switch(lean_obj_tag(v_e_17_))
+{
+case 0:
+{
+lean_object* v_a_22_; lean_object* v___x_23_; 
+lean_dec(v_h__4_21_);
+lean_dec(v_h__3_20_);
+lean_dec(v_h__2_19_);
+v_a_22_ = lean_ctor_get(v_e_17_, 0);
+lean_inc(v_a_22_);
+lean_dec_ref_known(v_e_17_, 1);
+v___x_23_ = lean_apply_1(v_h__1_18_, v_a_22_);
+return v___x_23_;
+}
+case 1:
+{
+lean_object* v_a_24_; lean_object* v___x_25_; 
+lean_dec(v_h__4_21_);
+lean_dec(v_h__3_20_);
+lean_dec(v_h__1_18_);
+v_a_24_ = lean_ctor_get(v_e_17_, 0);
+lean_inc_ref(v_a_24_);
+lean_dec_ref_known(v_e_17_, 1);
+v___x_25_ = lean_apply_1(v_h__2_19_, v_a_24_);
+return v___x_25_;
+}
+case 2:
+{
+lean_object* v_a_26_; lean_object* v_a_27_; lean_object* v___x_28_; 
+lean_dec(v_h__4_21_);
+lean_dec(v_h__2_19_);
+lean_dec(v_h__1_18_);
+v_a_26_ = lean_ctor_get(v_e_17_, 0);
+lean_inc_ref(v_a_26_);
+v_a_27_ = lean_ctor_get(v_e_17_, 1);
+lean_inc_ref(v_a_27_);
+lean_dec_ref_known(v_e_17_, 2);
+v___x_28_ = lean_apply_2(v_h__3_20_, v_a_26_, v_a_27_);
+return v___x_28_;
+}
+default: 
+{
+lean_object* v_a_29_; lean_object* v_a_30_; lean_object* v___x_31_; 
+lean_dec(v_h__3_20_);
+lean_dec(v_h__2_19_);
+lean_dec(v_h__1_18_);
+v_a_29_ = lean_ctor_get(v_e_17_, 0);
+lean_inc_ref(v_a_29_);
+v_a_30_ = lean_ctor_get(v_e_17_, 1);
+lean_inc_ref(v_a_30_);
+lean_dec_ref_known(v_e_17_, 2);
+v___x_31_ = lean_apply_2(v_h__4_21_, v_a_29_, v_a_30_);
+return v___x_31_;
+}
+}
+}
+}
+lean_object* initialize_Init(uint8_t builtin);
+lean_object* initialize_Init(uint8_t builtin);
+lean_object* initialize_LeanProofs_LeanProofs_Basic(uint8_t builtin);
+static bool _G_initialized = false;
+LEAN_EXPORT lean_object* initialize_LeanProofs_LeanProofs_exprDeterminism(uint8_t builtin) {
+lean_object * res;
+if (_G_initialized) return lean_io_result_mk_ok(lean_box(0));
+_G_initialized = true;
+res = initialize_Init(builtin);
+if (lean_io_result_is_error(res)) return res;
+lean_dec_ref(res);
+res = initialize_Init(builtin);
+if (lean_io_result_is_error(res)) return res;
+lean_dec_ref(res);
+res = initialize_LeanProofs_LeanProofs_Basic(builtin);
+if (lean_io_result_is_error(res)) return res;
+lean_dec_ref(res);
+return lean_io_result_mk_ok(lean_box(0));
+}
+#ifdef __cplusplus
+}
+#endif
